modify the definition of annotated command, add the VCG of hoare logic

Ann_Com.thy
@@ -5,28 +5,28 @@ begin
 type_synonym assn = "state \<Rightarrow> bool"
 
 datatype com =
-  Assign vname aexp      ("_ ::= _") |
+  Basic "state \<Rightarrow> state"      |
   Seq   com com          ("_;; _") |
   Cond bexp com com      ("IF _ THEN _ ELSE _ FI")|
   While bexp assn com    ("WHILE _ INV _ DO _ OD")|
   Wait bexp              ("WAIT _ END")
 
 datatype acom =
-  AAssign assn vname aexp       ("{_} _ ::= _") |
-  ASeq   acom acom              ("_;; _") |
+  ABasic assn "state \<Rightarrow> state"      |
+  ASeq   acom acom   ("_;; _") |
   ACond assn bexp acom acom     ("{_} IF _ THEN _ ELSE _ FI")|
   AWhile assn bexp assn acom    ("{_} WHILE _ INV _ DO _ OD")|
   AWait assn bexp              ("{_} WAIT _ END")
 
 fun pre :: "acom \<Rightarrow> assn" where
-"pre ({P} v ::= a) = P" |
+"pre (ABasic P f) = P" |
 "pre (c1;; c2) = pre(c1)" |
 "pre ({P} IF b THEN c1 ELSE c2 FI) = P"|
 "pre ({P} WHILE b INV I DO c OD) = P"|
 "pre ({P} WAIT b END) = P"
 
 fun strip::"acom \<Rightarrow> com" where
-"strip ({P} v ::= a) = (v ::= a)"|
+"strip (ABasic P f) = (Basic f)"|
 "strip (C1;; C2) = (strip(C1);; strip(C2))" |
 "strip ({P} IF b THEN C1 ELSE C2 FI) = (IF b THEN strip C1 ELSE strip C2 FI)"|
 "strip ({P} WHILE b INV I DO C OD) = (WHILE b INV I DO strip C OD)"|
