Example.thy
@@ -1,0 +1,17 @@
+theory Example
+imports Proof_Par
+begin
+
+abbreviation "wsum ==
+  Parallel [((Some (ABasic (\<lambda>s. s ''x'' = (0::int)) (\<lambda>s. s(''x'' := aval (Plus (V ''x'') (N 1)) s)))),(\<lambda>s. s ''x'' = aval (Plus (V ''x'') (N 1)) s)),
+    ((Some (ABasic (\<lambda>s. s ''x'' = (0::int)) (\<lambda>s. s(''x'' := aval (Plus (V ''x'') (N 1)) s)))),(\<lambda>s. s ''x'' = aval (Plus (V ''x'') (N 1)) s))]"
+
+subsubsection{* Proof by Hoare Logic *}
+
+text{* Note that we deal with sequences of commands from right to left,
+pulling back the postcondition towards the precondition. *}
+
+lemma "\<turnstile>\<^sub>P {\<lambda>s. s x = 0} wsum {\<lambda>s. s x = 2}"
+apply(rule PParallelE)
+
+end
